theories/simplang/examples/sum.v
@@ -9,28 +9,28 @@ From simuliris.simulation Require Import slsls lifting.
 Section fix_bi.
 Context (PROP : bi).
 Context {PROP_bupd : BiBUpd PROP}.
+Context {PROP_forall : BiPureForall PROP}.
 Context {PROP_affine : BiAffine PROP}.
 
-(* Sums are encoded as inj1 x -> (1, (1, x)); inj2 x -> (1, (2, x));
+(* TODO: maybe change into non-bijective thing?*)
+(* Sums are encoded as injL x -> (1, (1, x)); injR x -> (1, (2, x));
   the first tag encodes that this is a sum, the second tag the constructor.
   Pairs are now also tagged to force interpretation as a pair (instead of sum).
   (x, y) becomes (0, (x, y)).
  *)
 
-Definition inj1_enc : val := (LamV "x" (#1, (#1, "x"))).
-Definition inj2_enc : val := (LamV "x" (#1, (#2, "x"))).
+Definition inj1_enc : val := (λ: "x", (#1, "x"))%V.
+Definition inj2_enc : val := (λ: "x", (#2, "x"))%V.
 
 Definition diverge : val := (rec: "f" "x" := "f" "x")%V.
 
 (* on invalid inputs, we diverge: in the source we get stuck, so any target behaviour is okay *)
 Definition case_enc : val :=
-  (λ: "x" "f" "g", if: Fst "x" = #1 then
-    let: "x" := Snd "x" in
-    if: Fst "x" = #1 then "f" (Snd "x")
+  (λ: "x" "f" "g", 
+      if: Fst "x" = #1 then "f" (Snd "x")
       else if: Fst "x" = #2
         then "g" (Snd "x")
         else diverge #()
-    else diverge #()
   ).
 
 Definition case_prim : val :=
@@ -44,20 +44,21 @@ Definition case_prim : val :=
 Inductive val_rel_pure : val → val → Prop :=
   (* functions are never related *)
   | val_rel_lit l : val_rel_pure (LitV l) (LitV l)
-  | val_rel_injL v1 v2 : val_rel_pure v1 v2 → val_rel_pure ((#1, (#1, v1))%V) (InjLV v2)
-  | val_rel_injR v1 v2 : val_rel_pure v1 v2 → val_rel_pure ((#1, (#2, v1))%V) (InjRV v2)
+  | val_rel_injL v1 v2 : val_rel_pure v1 v2 → val_rel_pure ((#1, v1)%V) (InjLV v2)
+  | val_rel_injR v1 v2 : val_rel_pure v1 v2 → val_rel_pure ((#2, v1)%V) (InjRV v2)
   | val_rel_pair v1 v2 v1' v2' :
       val_rel_pure v1 v1' →
       val_rel_pure v2 v2' →
-      val_rel_pure ((#0, (v1, v2))%V) ((v1', v2')%V).
+      val_rel_pure ((v1, v2)%V) ((v1', v2')%V).
 Local Hint Constructors val_rel_pure : core.
 Definition val_rel_simp v1 v2 : PROP := (⌜val_rel_pure v1 v2⌝)%I.
 
-Instance sim_sum_lang : simul_lang PROP simp_lang :=
+(* TODO: make a Record ? *)
+Instance sim_sum_lang : SimulLang PROP simp_lang :=
   {|
     (* TODO *)
-    state_interp Pt σt Ps σs := ⌜ True ⌝%I;
-    val_rel := val_rel_simp
+    state_interp Pt σt Ps σs := True%I;
+    val_rel := val_rel_simp (* TODO: remove *)
   |}.
 Instance: Sim sim_sum_lang := sim_stutter.
 
@@ -74,77 +75,71 @@ Definition target_prog : gmap string ectx := {[ "mul2" := fun_to_ectx mul2_targe
 
 (** We want to prove: *)
 
-From iris.proofmode Require Import coq_tactics reduction.
-From iris.proofmode Require Export tactics.
-
 Lemma mul2_sim:
   ⊢ ∀ v_t v_s, val_rel v_t v_s -∗
-    mul2_target (of_val v_t) ⪯ mul2_source (of_val v_s) {{λ v_t' v_s', val_rel v_t' v_s' }}.
+    mul2_target (of_val v_t) ⪯ mul2_source (of_val v_s) {{ λ v_t' v_s', val_rel v_t' v_s' }}.
 Proof.
-  iIntros (??) "%". rewrite /mul2_target /mul2_source.
+  iIntros (?? Hval). rewrite /mul2_target /mul2_source.
   sim_pures.
   rewrite /case_enc /case_prim.
   sim_pures.
   (* TODO: automation for proving stuckness *)
-  inversion H; subst.
+  (* TODO: destruct *)
+  (* better: positive reasoning *) 
+  destruct Hval as [ l | v1 v2 Hval | v1 v2 Hval | ].
   - iApply sim_source_stuck. iIntros (????) "_". iPureIntro.
-    split; first done. intros e' σ' H0. inversion H0; subst.
-    (*clear H0. *)
-    (*induction K. *)
-    (*+ inv_head_step. *)
-    (*+ *)
+    split; first done. intros e' σ' Hprim. inversion Hprim; subst.
 
+    (* TODO: sep logic judgement for stuckness ; either 
+      * for every target, sim ...
+      * conclusion of sim_source_stuck with reach_stuck 
+
+
+      -> no inversions
+    *)
     admit.
   - sim_pures.
     sim_pures_target.
-    inversion H0; subst.
+    destruct Hval. 
     { destruct l.
-      * sim_pures. iModIntro. iPureIntro. constructor.
-      * iApply sim_source_stuck. admit.
-      * iApply sim_source_stuck. admit.
-      * iApply sim_source_stuck. admit.
-      * iApply sim_source_stuck. admit.
+      { sim_pures. iModIntro. iPureIntro. constructor. }
+      all: iApply sim_source_stuck; admit.
     }
     all: admit.
   - sim_pures. sim_pures_target.
-    inversion H0; subst.
+    destruct Hval.
     { destruct l.
-      * sim_pures. iModIntro. iPureIntro. constructor.
-      * iApply sim_source_stuck. admit.
-      * iApply sim_source_stuck. admit.
-      * iApply sim_source_stuck. admit.
-      * iApply sim_source_stuck. admit.
+      { sim_pures. iModIntro. iPureIntro. constructor. }
+      all: iApply sim_source_stuck; admit.
     }
     all: admit.
   - iApply sim_source_stuck. iIntros (????) "_". iPureIntro.
     split; first done. intros e' σ' H2. inversion H2; subst.
     admit.
-
 Admitted.
 
 
 (* TODO move *)
-Lemma step_Call e_t e_s (v_t v_s : val) f :
+Lemma step_call e_t e_s (v_t v_s : val) f :
   to_val e_t = Some v_t → to_val e_s = Some v_s →
-  ⊢ val_rel v_t v_s -∗ Call f e_t ⪯ Call f e_s {{val_rel}}.
+  ⊢ val_rel v_t v_s -∗ Call (of_fname f) e_t ⪯ Call (of_fname f) e_s {{ val_rel }}.
 Proof.
   intros <-%of_to_val <-%of_to_val.
   iIntros "H". rewrite sim_unfold. iIntros (????) "[H1 H2]". iModIntro.
   iRight; iRight. iExists f, empty_ectx, v_t, empty_ectx, v_s, σ_s. cbn. iFrame.
-  iSplitL ""; first done. iSplitL "". { iPureIntro. constructor. }
+  iSplitR; first done. iSplitR. { iPureIntro. constructor. }
   iIntros (v_t' v_s' ) "H". iApply sim_value. iApply "H".
 Qed.
 
-Definition source_client := (λ: "x", Call "mul2" (InjL "x"))%V.
-Definition target_client := (λ: "x", Call "mul2" (inj1_enc "x"))%V.
+Definition source_client := (λ: "x", Call (of_fname "mul2") (InjL "x"))%V.
+Definition target_client := (λ: "x", Call (of_fname "mul2") (inj1_enc "x"))%V.
 
 Lemma client_sim (n : Z) :
-  ⊢ target_client #n ⪯ source_client #n {{λ v_t v_s, val_rel v_t v_s }}.
+  ⊢ target_client #n ⪯ source_client #n {{ λ v_t v_s, val_rel v_t v_s }}.
 Proof.
   iStartProof. rewrite /target_client /source_client.
   sim_pures. sim_bind (inj1_enc #n) (InjL #n).
   rewrite /inj1_enc.
   sim_pures. sim_pures_target.
-  iApply step_Call; eauto.
+  iApply step_call; eauto.
 Qed.
-
